src/ORSet.thy
@@ -17,14 +17,13 @@ definition interpret_op :: "('id, 'a) operation \<Rightarrow> ('id, 'a) state \<
          after  = case oper of Add i e \<Rightarrow> before \<union> {i} | Rem is e \<Rightarrow> before - is
      in  Some (state ((op_elem oper) := after))"
     
-definition valid_behaviours :: "(('id, 'a) operation \<Rightarrow> 'id) \<Rightarrow> ('id, 'a) state \<Rightarrow> ('id, 'a) operation \<Rightarrow> bool" where
-  "valid_behaviours msg_id state oper \<equiv>
-     case oper of
-       Add i  e \<Rightarrow> i = msg_id oper
-     | Rem is e \<Rightarrow> is = state e"
-  
-locale orset = network_with_constrained_ops msg_id history interpret_op "\<lambda>x. {}" "valid_behaviours msg_id"
-  for msg_id :: "('id, 'a) operation \<Rightarrow> 'id" and history :: "nat \<Rightarrow> ('id, 'a) operation event list"
+definition valid_behaviours :: "('id, 'a) state \<Rightarrow> 'id \<times> ('id, 'a) operation \<Rightarrow> bool" where
+  "valid_behaviours state msg \<equiv>
+     case msg of
+       (i, Add j  e) \<Rightarrow> i = j |
+       (i, Rem is e) \<Rightarrow> is = state e"
+
+locale orset = network_with_constrained_ops _ interpret_op "\<lambda>x. {}" valid_behaviours
 
 lemma (in orset) add_add_commute:
   shows "\<langle>Add i1 e1\<rangle> \<rhd> \<langle>Add i2 e2\<rangle> = \<langle>Add i2 e2\<rangle> \<rhd> \<langle>Add i1 e1\<rangle>"
@@ -34,10 +33,7 @@ lemma (in orset) add_rem_commute:
   assumes "i \<notin> is"
   shows "\<langle>Add i e1\<rangle> \<rhd> \<langle>Rem is e2\<rangle> = \<langle>Rem is e2\<rangle> \<rhd> \<langle>Add i e1\<rangle>"
   using assms by(auto simp add: interpret_op_def kleisli_def op_elem_def, fastforce)
-  
-definition (in orset) added_ids :: "('id, 'a) operation event list \<Rightarrow> 'a \<Rightarrow> 'id list" where
-  "added_ids es p \<equiv> List.map_filter (\<lambda>x. case x of Deliver (Add i e) \<Rightarrow> if e = p then Some i else None | _ \<Rightarrow> None) es"
-    
+
 lemma (in orset) apply_operations_never_fails:
   assumes "xs prefix of i"
   shows "apply_operations xs \<noteq> None"
@@ -46,9 +42,21 @@ lemma (in orset) apply_operations_never_fails:
    apply clarsimp
   apply(case_tac "x"; clarsimp)
    apply force
-  using interpret_op_def apply (metis bind.bind_lunit prefix_of_appendD)
+  apply(metis interpret_op_def interp_msg_def bind.bind_lunit prefix_of_appendD)
   done
-    
+
+lemma (in orset) add_id_valid:
+  assumes "xs prefix of j"
+    and "Deliver (i1, Add i2 e) \<in> set xs"
+  shows "i1 = i2"
+  apply(subgoal_tac "\<exists>state. valid_behaviours state (i1, Add i2 e)")
+  apply(simp add: valid_behaviours_def)
+  using assms deliver_in_prefix_is_valid apply blast
+done
+
+definition (in orset) added_ids :: "('id \<times> ('id, 'b) operation) event list \<Rightarrow> 'b \<Rightarrow> 'id list" where
+  "added_ids es p \<equiv> List.map_filter (\<lambda>x. case x of Deliver (i, Add j e) \<Rightarrow> if e = p then Some j else None | _ \<Rightarrow> None) es"
+
 lemma (in orset) [simp]:
   shows "added_ids [] e = []"
   by (auto simp: added_ids_def map_filter_def)
@@ -62,17 +70,22 @@ lemma (in orset) added_ids_Broadcast_collapse [simp]:
   by (auto simp: added_ids_def map_filter_append map_filter_def)
     
 lemma (in orset) added_ids_Deliver_Rem_collapse [simp]:
-  shows "added_ids ([Deliver (Rem is e)]) e' = []"
+  shows "added_ids ([Deliver (i, Rem is e)]) e' = []"
   by (auto simp: added_ids_def map_filter_append map_filter_def)
     
 lemma (in orset) added_ids_Deliver_Add_diff_collapse [simp]:
-  shows "e \<noteq> e' \<Longrightarrow> added_ids ([Deliver (Add i e)]) e' = []"
+  shows "e \<noteq> e' \<Longrightarrow> added_ids ([Deliver (i, Add j e)]) e' = []"
   by (auto simp: added_ids_def map_filter_append map_filter_def)
     
 lemma (in orset) added_ids_Deliver_Add_same_collapse [simp]:
-  shows "added_ids ([Deliver (Add i e)]) e = [i]"
+  shows "added_ids ([Deliver (i, Add j e)]) e = [j]"
   by (auto simp: added_ids_def map_filter_append map_filter_def)
-    
+
+lemma (in orset) added_id_not_in_set:
+  assumes "i1 \<notin> set (added_ids [Deliver (i, Add i2 e)] e)"
+  shows "i1 \<noteq> i2"
+  using assms by simp
+
 lemma (in orset) apply_operations_added_ids:
   assumes "es prefix of j"
     and "apply_operations es = Some f"
@@ -84,41 +97,43 @@ lemma (in orset) apply_operations_added_ids:
    apply clarsimp
    apply force
   apply clarsimp
-  apply (case_tac x2)
-   apply clarsimp
+  apply (case_tac b)
    apply(subgoal_tac "xs prefix of j", clarsimp split: bind_splits)
+   apply(clarsimp simp add: interp_msg_def)
     apply(erule_tac x="xb" in meta_allE, clarsimp simp add: interpret_op_def)
-    apply(clarsimp split: if_split_asm simp add: op_elem_def)
+    apply(clarsimp split: if_split_asm simp add: op_elem_def added_id_not_in_set)
      apply force
     apply force
    apply force
   apply(subgoal_tac "xs prefix of j", clarsimp split: bind_splits)
-   apply(erule_tac x="xb" in meta_allE, clarsimp simp add: interpret_op_def)
+   apply(erule_tac x="xb" in meta_allE, clarsimp simp add: interpret_op_def interp_msg_def)
    apply(clarsimp split: if_split_asm simp add: op_elem_def)
     apply force
    apply force
   apply force
 done
-    
+
 lemma (in orset) Deliver_added_ids:
-  assumes "i \<in> set (added_ids xs e)"
-  shows "Deliver (Add i e) \<in> set xs"
+  assumes "xs prefix of j"
+    and "i \<in> set (added_ids xs e)"
+  shows "Deliver (i, Add i e) \<in> set xs"
     using assms
   apply (induct xs rule: rev_induct)
      apply clarsimp
     apply (case_tac x)
-     apply clarsimp
+     apply(simp add: prefix_of_appendD)
     apply clarsimp
-    apply (case_tac x2)
+    apply (case_tac b)
      apply clarsimp
-      apply (metis added_ids_Deliver_Add_diff_collapse added_ids_Deliver_Add_same_collapse empty_iff list.set(1) set_ConsD)
-     apply clarsimp
+     apply (metis added_ids_Deliver_Add_diff_collapse added_ids_Deliver_Add_same_collapse
+       empty_iff list.set(1) set_ConsD add_id_valid in_set_conv_decomp prefix_of_appendD)
+    apply (metis added_ids_Deliver_Rem_collapse empty_iff list.set(1) prefix_of_appendD)
     done
-      
+
 lemma (in orset) Broadcast_Deliver_prefix_closed:
-  assumes "xs @ [Broadcast (Rem ix e)] prefix of j"
+  assumes "xs @ [Broadcast (r, Rem ix e)] prefix of j"
     and "i \<in> ix"
-  shows "Deliver (Add i e) \<in> set xs"
+  shows "Deliver (i, Add i e) \<in> set xs"
   using assms
   apply(subgoal_tac "\<exists>y. apply_operations xs = Some y")
    apply clarsimp
@@ -128,15 +143,16 @@ lemma (in orset) Broadcast_Deliver_prefix_closed:
      apply force
     apply(clarsimp)
   using Deliver_added_ids apply blast
-   apply (metis (mono_tags) broadcast_only_valid_ops operation.case(2) option.simps(1) valid_behaviours_def)
-    using broadcast_only_valid_ops by blast
+   apply (metis (mono_tags, lifting) broadcast_only_valid_msgs operation.case(2) option.simps(1)
+     valid_behaviours_def case_prodD)
+  using broadcast_only_valid_msgs apply blast
+  done
 
-  
 lemma (in orset) Broadcast_Deliver_prefix_closed2:
   assumes "xs prefix of j"
-    and "Broadcast (Rem ix e) \<in> set xs"
+    and "Broadcast (r, Rem ix e) \<in> set xs"
     and "i \<in> ix"
-  shows "Deliver (Add i e) \<in> set xs"
+  shows "Deliver (i, Add i e) \<in> set xs"
   using assms
   apply(induction xs rule: rev_induct)
    apply clarsimp
@@ -148,37 +164,37 @@ lemma (in orset) Broadcast_Deliver_prefix_closed2:
   apply clarsimp
     using Broadcast_Deliver_prefix_closed apply metis
 done
-    
+
 lemma (in orset) concurrent_add_remove_independent_technical:
   assumes "i \<in> is"
     and "xs prefix of j"
-    and "Add i e \<in> set (node_deliver_messages xs)" and "Rem is e \<in> set (node_deliver_messages xs)"
-  shows "hb (Add i e) (Rem is e)"
+    and "(i, Add i e) \<in> set (node_deliver_messages xs)" and "(ir, Rem is e) \<in> set (node_deliver_messages xs)"
+  shows "hb (i, Add i e) (ir, Rem is e)"
     using assms
-  apply(subgoal_tac "\<exists>pre k. pre@[Broadcast (Rem is e)] prefix of k")
+  apply(subgoal_tac "\<exists>pre k. pre@[Broadcast (ir, Rem is e)] prefix of k")
    apply clarsimp
-     apply(frule broadcast_only_valid_ops, clarsimp simp add: valid_behaviours_def)
-     apply(subgoal_tac "Deliver (Add i e) \<in> set pre")
+     apply(frule broadcast_only_valid_msgs, clarsimp simp add: valid_behaviours_def)
+     apply(subgoal_tac "Deliver (i, Add i e) \<in> set pre")
       apply(rule_tac i=k in hb.intros(2))
     using events_in_local_order apply blast
      apply(insert Broadcast_Deliver_prefix_closed2)
-     apply(erule_tac x="pre @ [Broadcast (Rem (state e) e)]" in meta_allE)
-     apply(erule_tac x=k in meta_allE, erule_tac x="is" in meta_allE)
+     apply(erule_tac x="pre @ [Broadcast (ir, Rem (state e) e)]" in meta_allE)
+     apply(erule_tac x=k in meta_allE, erule_tac x=ir in meta_allE, erule_tac x="is" in meta_allE)
      apply(erule_tac x="e" in meta_allE, erule_tac x=i in meta_allE)
       apply clarsimp
     using delivery_has_a_cause events_before_exist prefix_msg_in_history apply blast
     done
-      
+
 lemma (in orset) Deliver_Add_same_id_same_message:
-  assumes "Deliver (Add i e1) \<in> set (history j)" and "Deliver (Add i e2) \<in> set (history j)"
+  assumes "Deliver (i, Add i e1) \<in> set (history j)" and "Deliver (i, Add i e2) \<in> set (history j)"
   shows "e1 = e2"
-  apply(subgoal_tac "\<exists>pre k. pre@[Broadcast (Add i e1)] prefix of k")
-   apply(subgoal_tac "\<exists>pre k. pre@[Broadcast (Add i e2)] prefix of k")
+  apply(subgoal_tac "\<exists>pre k. pre@[Broadcast (i, Add i e1)] prefix of k")
+   apply(subgoal_tac "\<exists>pre k. pre@[Broadcast (i, Add i e2)] prefix of k")
     apply clarsimp
-    apply(subgoal_tac "Broadcast (Add i e1) \<in> set (history k)")
-    apply(subgoal_tac "Broadcast (Add i e2) \<in> set (history ka)")
+    apply(subgoal_tac "Broadcast (i, Add i e1) \<in> set (history k)")
+    apply(subgoal_tac "Broadcast (i, Add i e2) \<in> set (history ka)")
     apply(drule msg_id_unique, assumption)
-       apply(drule broadcast_only_valid_ops)+
+       apply(drule broadcast_only_valid_msgs)+
        apply(clarsimp simp add: valid_behaviours_def)
       apply force
   using prefix_of_node_history_def apply(metis Un_insert_right insert_subset list.simps(15) prefix_to_carriers set_append)
@@ -190,13 +206,13 @@ lemma (in orset) Deliver_Add_same_id_same_message:
 lemma (in orset) ids_imply_messages_same:
   assumes "i \<in> is"
     and "xs prefix of j"
-    and "Add i e1 \<in> set (node_deliver_messages xs)" and "Rem is e2 \<in> set (node_deliver_messages xs)"
+    and "(i, Add i e1) \<in> set (node_deliver_messages xs)" and "(ir, Rem is e2) \<in> set (node_deliver_messages xs)"
   shows "e1 = e2"
   using assms
-      apply(subgoal_tac "\<exists>pre k. pre@[Broadcast (Rem is e2)] prefix of k")
+      apply(subgoal_tac "\<exists>pre k. pre@[Broadcast (ir, Rem is e2)] prefix of k")
    apply clarsimp
-     apply(frule broadcast_only_valid_ops, clarsimp simp add: valid_behaviours_def)
-   apply(subgoal_tac "Deliver (Add i e2) \<in> set pre")
+     apply(frule broadcast_only_valid_msgs, clarsimp simp add: valid_behaviours_def)
+   apply(subgoal_tac "Deliver (i, Add i e2) \<in> set pre")
     apply(rule_tac j=j and i=i in Deliver_Add_same_id_same_message)
   using prefix_msg_in_history apply blast
   using causal_broadcast events_in_local_order local_order_prefix_closed prefix_contains_msg prefix_to_carriers apply blast
@@ -205,12 +221,12 @@ lemma (in orset) ids_imply_messages_same:
   done
 
 corollary (in orset) concurrent_add_remove_independent:
-  assumes "\<not> hb (Add i e1) (Rem is e2)" and "\<not> hb (Rem is e2) (Add i e1)"
+  assumes "\<not> hb (i, Add i e1) (ir, Rem is e2)" and "\<not> hb (ir, Rem is e2) (i, Add i e1)"
     and "xs prefix of j"
-    and "Add i e1 \<in> set (node_deliver_messages xs)" and "Rem is e2 \<in> set (node_deliver_messages xs)"
+    and "(i, Add i e1) \<in> set (node_deliver_messages xs)" and "(ir, Rem is e2) \<in> set (node_deliver_messages xs)"
   shows "i \<notin> is"
   using assms ids_imply_messages_same concurrent_add_remove_independent_technical by fastforce
-                                        
+
 lemma (in orset) rem_rem_commute:
   shows "\<langle>Rem i1 e1\<rangle> \<rhd> \<langle>Rem i2 e2\<rangle> = \<langle>Rem i2 e2\<rangle> \<rhd> \<langle>Rem i1 e1\<rangle>"
   by(unfold interpret_op_def op_elem_def kleisli_def, fastforce)
@@ -220,10 +236,14 @@ lemma (in orset) concurrent_operations_commute:
   shows "hb.concurrent_ops_commute (node_deliver_messages xs)"
   using assms
   apply(clarsimp simp: hb.concurrent_ops_commute_def)
-  apply(case_tac "x"; case_tac "y")
-  apply(auto simp add: hb.concurrent_def add_add_commute add_rem_commute rem_rem_commute concurrent_add_remove_independent)
+  apply(unfold interp_msg_def, simp)
+  apply(case_tac "b"; case_tac "ba")
+  apply(simp add: add_add_commute hb.concurrent_def)
+  apply(metis add_rem_commute concurrent_add_remove_independent hb.concurrent_def add_id_valid prefix_contains_msg)
+  apply(metis add_rem_commute concurrent_add_remove_independent hb.concurrent_def add_id_valid prefix_contains_msg)
+  apply(simp add: rem_rem_commute hb.concurrent_def)
   done
-  
+
 theorem (in orset) convergence:
   assumes "set (node_deliver_messages xs) = set (node_deliver_messages ys)"
       and "xs prefix of i" and "ys prefix of j"
@@ -233,12 +253,14 @@ using assms by(auto simp add: apply_operations_def intro: hb.convergence_ext con
               
 context orset begin
 
-sublocale sec: strong_eventual_consistency weak_hb hb interpret_op
+sublocale sec: strong_eventual_consistency weak_hb hb interp_msg
   "\<lambda>ops.\<exists>xs i. xs prefix of i \<and> node_deliver_messages xs = ops" "\<lambda>x.{}"
   apply(standard; clarsimp)
-      apply(auto simp add: hb_consistent_prefix node_deliver_messages_distinct concurrent_operations_commute)
-   apply (metis (no_types, lifting) interpret_op_def)
-    using drop_last_message apply blast
+      apply(auto simp add: hb_consistent_prefix node_deliver_messages_distinct
+        concurrent_operations_commute)
+   apply(metis (no_types, lifting) apply_operations_def bind.bind_lunit not_None_eq
+     hb.apply_operations_Snoc kleisli_def apply_operations_never_fails interp_msg_def)
+  using drop_last_message apply blast
 done
 
 end
